

System of ODEsSolve:

$$\dot{X} = \underbrace{\begin{pmatrix} 1 & -2 & 2 \\ -2 & 1 & -2 \\ 2 & -2 & 1 \end{pmatrix}}_A X$$

Soln:

$$|(A - \lambda I)| = 0$$

$$\left| \begin{pmatrix} 1 & -2 & 2 \\ -2 & 1 & -2 \\ 2 & -2 & 1 \end{pmatrix} - \begin{pmatrix} \lambda & 0 & 0 \\ 0 & \lambda & 0 \\ 0 & 0 & \lambda \end{pmatrix} \right| = 0$$

$$\checkmark \quad \begin{vmatrix} (1-\lambda) & -2 & 2 \\ -2 & (1-\lambda) & -2 \\ 2 & -2 & (1-\lambda) \end{vmatrix} = 0$$

$$\Rightarrow (1-\lambda) \left[(1-\lambda)(1-\lambda) - 4 \right] + 2 \left[-2(1-\lambda) + 4 \right] + 2 \left[4 - 2(1-\lambda) \right] = 0$$

$$\Rightarrow (1-\lambda) (1-2\lambda+\lambda^2-4) + 2(-2+2\lambda+4) + 2(4-2+2\lambda) = 0$$

$$\Rightarrow (1-\lambda) (\lambda^2-2\lambda-3) + 4(\lambda+1) + 4(\lambda+1) = 0$$

$$\Rightarrow (1-\lambda) (\lambda-3)(\lambda+1) + 8(\lambda+1) = 0$$

$$(\lambda+1) [(1-\lambda)(\lambda-3) + 8] = 0$$

$$(\lambda+1) (\lambda - \lambda^2 - 3 + 3\lambda + 8)$$

$$(\lambda+1) (-\lambda^2 + 4\lambda + 5)$$

$$- (\lambda+1) (\lambda^2 - 4\lambda - 5) = 0$$

$$- (\lambda+1) (\lambda^2 - 5\lambda + \lambda - 5) = 0$$

$$- (\lambda+1) (\lambda-5)(\lambda+1) = 0$$

$$\boxed{\lambda = -1, -1, 5}$$

For $\lambda = -1$, we find the eigenvector: K

$$(A - \lambda I)K = 0$$

$$\begin{bmatrix} 1-(-1) & -2 & 2 \\ -2 & 1-(-1) & -2 \\ 2 & -2 & 1-(-1) \end{bmatrix} \begin{bmatrix} k_1 \\ k_2 \\ k_3 \end{bmatrix} = \begin{pmatrix} 0 \\ 0 \\ 0 \end{pmatrix}$$

$$\begin{pmatrix} 2 & -2 & 2 \\ -2 & 2 & -2 \\ 2 & -2 & 2 \end{pmatrix} \begin{pmatrix} k_1 \\ k_2 \\ k_3 \end{pmatrix} = \begin{pmatrix} 0 \\ 0 \\ 0 \end{pmatrix}$$

$$R_3^{\text{new}} = R_3 + R_2$$

$$\approx \begin{pmatrix} 2 & -2 & 2 \\ -2 & 2 & -2 \\ 0 & 0 & 0 \end{pmatrix} \begin{pmatrix} k_1 \\ k_2 \\ k_3 \end{pmatrix} = \begin{pmatrix} 0 \\ 0 \\ 0 \end{pmatrix}$$

$$R_2^{\text{new}} = R_2 + R_1$$

$$\approx \begin{pmatrix} 2 & -2 & 2 \\ 0 & 0 & 0 \\ 0 & 0 & 0 \end{pmatrix} \begin{pmatrix} k_1 \\ k_2 \\ k_3 \end{pmatrix} = \begin{pmatrix} 0 \\ 0 \\ 0 \end{pmatrix}$$

We have Two free variables.

→ let k_2 & k_3 free variables.

$$\begin{aligned} \rightarrow \underline{k_2 = 1, \quad k_3 = 0} & \Rightarrow 2k_1 - 2k_2 + 2k_3 = 0 \\ & 2k_1 - 2 + 0 = 0 \\ & k_1 = 1 \end{aligned}$$

$$\therefore K = \begin{pmatrix} 1 \\ 1 \\ 0 \end{pmatrix} \leftarrow$$

$$\begin{aligned} \underline{\text{Also,}} \quad \text{let } k_3 = 1 \quad \& \quad k_2 = 0 \Rightarrow 2k_1 - 2k_2 + 2k_3 = 0 \\ & 2k_1 - 2 \cdot 0 + 2 \cdot 1 = 0 \\ & k_1 = -1 \end{aligned}$$

$$K = \begin{pmatrix} -1 \\ 0 \\ 1 \end{pmatrix} \leftarrow$$

Also, for $\lambda = 5$, we find the eigenvector K as:

$$\begin{pmatrix} 1-5 & -2 & 2 \\ -2 & 1-5 & -2 \\ 2 & -2 & 1-5 \end{pmatrix} \begin{pmatrix} k_1 \\ k_2 \\ k_3 \end{pmatrix} = \begin{pmatrix} 0 \\ 0 \\ 0 \end{pmatrix}$$

$$\Rightarrow \begin{pmatrix} -4 & -2 & 2 \\ -2 & -4 & -2 \\ \textcircled{2} & -2 & -4 \end{pmatrix} \begin{pmatrix} k_1 \\ k_2 \\ k_3 \end{pmatrix} = \begin{pmatrix} 0 \\ 0 \\ 0 \end{pmatrix}$$

$R_3^{\text{new}} = R_3 + R_2$
 \approx

$$\begin{pmatrix} -4 & -2 & 2 \\ -2 & -4 & -2 \\ \textcircled{-2} & -6 & -6 \end{pmatrix} \begin{pmatrix} k_1 \\ k_2 \\ k_3 \end{pmatrix} = \begin{pmatrix} 0 \\ 0 \\ 0 \end{pmatrix}$$

$R_2^{\text{new}} = 2R_2 - R_1$
 \approx

$$\begin{pmatrix} -4 & -2 & 2 \\ 0 & -6 & -6 \\ 0 & \textcircled{-6} & -6 \end{pmatrix} \begin{pmatrix} k_1 \\ k_2 \\ k_3 \end{pmatrix} = \begin{pmatrix} 0 \\ 0 \\ 0 \end{pmatrix}$$

\approx

$$\begin{pmatrix} -4 & -2 & 2 \\ 0 & -6 & -6 \\ 0 & 0 & 0 \end{pmatrix} \begin{pmatrix} k_1 \\ k_2 \\ k_3 \end{pmatrix} = \begin{pmatrix} 0 \\ 0 \\ 0 \end{pmatrix}$$

Let k_3 be free variable. & $k_3 = 2$

$$\therefore -6k_2 - 6k_3 = 0$$

$$-6k_2 - 6 \times 2 = 0$$

$$k_2 = -2$$

\mathcal{L}

$$-4k_1 - 2k_2 + 2k_3 = 0$$

$$-4k_1 - 2(-2) + 2(2) = 0$$

$$-4k_1 + 4 + 4 = 0$$

$$-4k_1 = -8,$$

$$k_1 = 2$$

$$K = \begin{pmatrix} 2 \\ -2 \\ 2 \end{pmatrix}$$

General solution:

$$X = c_1 \begin{pmatrix} 1 \\ 1 \\ 0 \end{pmatrix} e^{-t} + c_2 \begin{pmatrix} -1 \\ 0 \\ 1 \end{pmatrix} e^{-t} + c_3 \begin{pmatrix} 2 \\ -2 \\ 2 \end{pmatrix} e^{5t}$$

Ans

Chp# 8.3

Non-Homogeneous ODE

$$\dot{X} = AX + F(t), \quad F(t) \neq 0$$

In this case, the general solution X

$$X = X_c + X_p$$

X_c : comes by solving the Homogeneous part.

X_p : various process

- (i) Superposition
- (ii) Variation of parameters.

Ex: Solve: $\dot{X} = \begin{pmatrix} 6 & 1 \\ 4 & 3 \end{pmatrix} X + \underbrace{\begin{pmatrix} 6t \\ -10t + 4 \end{pmatrix}}_{\uparrow F(t)}$

Sol

General solution:

$$X = X_c + X_p$$

For X_c : we solve: $\dot{X} = \begin{pmatrix} 6 & 1 \\ 4 & 3 \end{pmatrix} X$

$$\lambda = 2, 7 \quad \begin{matrix} \swarrow & \searrow \\ K = \begin{pmatrix} -1/4 \\ 1 \end{pmatrix} & K = \begin{pmatrix} -1 \\ -1 \end{pmatrix} \end{matrix}$$

$$X_c = c_1 \begin{pmatrix} -\frac{1}{4} \\ 1 \end{pmatrix} e^{2t} + c_2 \begin{pmatrix} -1 \\ -1 \end{pmatrix} e^{7t}$$

For X_p : we follow the superposition method:

$$\begin{aligned} F(t) &= \begin{pmatrix} 6t \\ -10t + 4 \end{pmatrix} \\ &= \underbrace{\begin{pmatrix} 6 \\ -10 \end{pmatrix}}_A t + \underbrace{\begin{pmatrix} 0 \\ 4 \end{pmatrix}}_B \end{aligned}$$

$$\therefore X_p = At + B$$

$$X_p = \underbrace{\begin{pmatrix} a_1 \\ a_2 \end{pmatrix}}_A t + \underbrace{\begin{pmatrix} b_1 \\ b_2 \end{pmatrix}}_B \quad \leftarrow$$

So, $X_p' = \underline{A} X_p + F(t)$

$$\underbrace{\begin{pmatrix} a_1 \\ a_2 \end{pmatrix}}_{X_p} = \underbrace{\begin{pmatrix} 6 & 1 \\ 4 & 3 \end{pmatrix}}_A \underbrace{\left[\begin{pmatrix} a_1 \\ a_2 \end{pmatrix} t + \begin{pmatrix} b_1 \\ b_2 \end{pmatrix} \right]}_{X(p)} + \underbrace{\begin{pmatrix} 6t \\ -10t + 4 \end{pmatrix}}_{F(t)}$$

$$\begin{pmatrix} a_1 \\ a_2 \end{pmatrix} = \begin{pmatrix} 6 & 1 \\ 4 & 3 \end{pmatrix} \begin{pmatrix} a_1 t + b_1 \\ a_2 t + b_2 \end{pmatrix} + \begin{pmatrix} 6t \\ -10t + 4 \end{pmatrix}$$

$$\begin{pmatrix} a_1 \\ a_2 \end{pmatrix} = \begin{pmatrix} 6a_1 t + 6b_1 + a_2 t + b_2 + 6t \\ 4a_1 t + 4b_1 + 3a_2 t + 3b_2 - 10t + 4 \end{pmatrix}$$

$$\begin{pmatrix} a_1 \\ a_2 \end{pmatrix} = \begin{bmatrix} (6a_1 + a_2 + 6)t + (6b_1 + b_2) \\ (4a_1 + 3a_2 - 10)t + (4b_1 + 3b_2 + 4) \end{bmatrix}$$

Equating coefficient from both sides:

$$\begin{bmatrix} 6a_1 + a_2 + 6 = 0 \\ 4a_1 + 3a_2 - 10 = 0 \end{bmatrix}$$

$$\begin{bmatrix} 6b_1 + b_2 = \cancel{a_1} - 2 \\ 4b_1 + 3b_2 + 4 = \cancel{a_2} 6 \end{bmatrix}$$

↓

solve:

$$a_1 = -2$$

$$a_2 = 6$$

solve:

$$b_1 = -4/7$$

$$b_2 = 10/7$$

$$\begin{aligned} X_p &= \begin{pmatrix} a_1 \\ a_2 \end{pmatrix} t + \begin{pmatrix} b_1 \\ b_2 \end{pmatrix} \\ &= \begin{pmatrix} -2 \\ 6 \end{pmatrix} t + \begin{pmatrix} -4/7 \\ 10/7 \end{pmatrix} \end{aligned}$$

$$X = X_c + X_p$$

$$= c_1 \begin{pmatrix} -1/4 \\ 1 \end{pmatrix} e^{2t} + c_2 \begin{pmatrix} -1 \\ -1 \end{pmatrix} e^{7t}$$

$$+ \begin{pmatrix} -2 \\ 6 \end{pmatrix} t + \begin{pmatrix} -4/7 \\ 10/7 \end{pmatrix}$$

Ans